src/crypto_foundations/computational_monads/random_oracle.lean
@@ -1,17 +1,26 @@
 import crypto_foundations.computational_monads.oracle_comp
 
--- def random_simulation {spec : oracle_comp_spec}
+open oracle_comp oracle_comp_spec
 
-@[derive comp.is_well_formed]
-def oracle_comp.simulate_random_oracle {T U C : Type}
-  [decidable_eq T] [fintype U] [inhabited U]
-  (oc : oracle_comp (oracle_comp_spec.singleton_spec T U) C)
-  [oc.is_well_formed] (log_init : list (T × U)) :=
-oc.simulate log_init (λ _ log t, 
-  option.rec_on (log.find (λ tu, t = tu.1)) 
-  -- If this isn't in the query log, return a random output and add that to the log
-    (comp.bind (comp.rnd U) (λ u, comp.ret ⟨u, ⟨t, u⟩ :: log⟩))
-    (λ tu, comp.ret ⟨tu.2, log⟩))
+def random_simulation_oracle (T U : Type) 
+  [decidable_eq T] [fintype U] [inhabited U] :
+  simulation_oracle (singleton_spec T U) :=
+{ S := list (T × U),
+  o := λ _ log t, option.rec_on (log.find (λ tu, t = tu.1)) 
+    ((comp.bind (comp.rnd U) (λ u, comp.ret ⟨u, ⟨t, u⟩ :: log⟩)))
+    ((λ tu, comp.ret ⟨tu.2, log⟩)),
+  oracle_is_well_formed := by apply_instance }
+
+-- @[derive comp.is_well_formed]
+-- def oracle_comp.simulate_random_oracle {T U C : Type}
+--   [decidable_eq T] [fintype U] [inhabited U]
+--   (oc : oracle_comp (oracle_comp_spec.singleton_spec T U) C)
+--   [oc.is_well_formed] (log_init : list (T × U)) :=
+-- oc.simulate log_init (λ _ log t, 
+--   option.rec_on (log.find (λ tu, t = tu.1)) 
+--   -- If this isn't in the query log, return a random output and add that to the log
+--     (comp.bind (comp.rnd U) (λ u, comp.ret ⟨u, ⟨t, u⟩ :: log⟩))
+--     (λ tu, comp.ret ⟨tu.2, log⟩))
 
 -- def random_simulation {T U C : Type} 
 --   [decidable_eq T] [fintype U] [inhabited U]
